WIP

cava/Cava/Semantics/Simulation.v
@@ -14,6 +14,7 @@
 (* limitations under the License.                                           *)
 (****************************************************************************)
 
+Require Import Coq.Arith.PeanoNat.
 Require Import Coq.Lists.List.
 Require Import Coq.micromega.Lia.
 Require Import coqutil.Tactics.Tactics.
@@ -27,58 +28,49 @@ Require Import Cava.Util.Identity.
 
 Existing Instance CombinationalSemantics.
 
-(* Run a circuit for many timesteps, starting at the reset value *)
-Definition simulate {i o} (c : Circuit i o) (input : list i) : list o :=
+Fixpoint simulate_with_state {i o} (c : Circuit i o) (st : circuit_state c) (input : list i)
+  : list o * list (circuit_state c) :=
+  match input with
+  | [] => ([], [])
+  | i :: input =>
+    let o_st := step c st i in
+    let out_states := simulate_with_state c (snd o_st) input in
+    (fst o_st :: fst out_states, snd o_st :: snd out_states)
+  end.
+
+(*
+Fixpoint simulate_init {i o} (c : Circuit i o) (st : circuit_state c) (input : list i) : list o :=
   match input with
   | [] => []
   | i :: input =>
-    let '(o,st) := step c (reset_state c) i in
-    let '(acc, _) := fold_left_accumulate
-                       (fun o_st => step c (snd o_st))
-                       input (o,st) in
-    map fst acc
-  end.
+    let o_st := step c st i in
+    fst o_st :: simulate_init c (snd o_st) input
+  end.*)
+
+(* Run a circuit for many timesteps, starting at the reset value *)
+Definition simulate {i o} (c : Circuit i o) (input : list i) : list o :=
+  fst (simulate_with_state c (reset_state c) input).
+
+Local Ltac simsimpl :=
+  repeat first [ progress cbv [simulate]
+               | progress cbn [reset_state circuit_state simulate_with_state step fst snd]
+               | destruct_pair_let
+               | progress simpl_ident ].
 
 Lemma simulate_compose {A B C} (c1 : Circuit A B) (c2 : Circuit B C) (input : list A) :
   simulate (Compose c1 c2) input = simulate c2 (simulate c1 input).
 Proof.
-  clear.
-  cbv [simulate]. destruct input as [|i0 input]; [ reflexivity | ].
-  repeat destruct_pair_let.
-  destruct input as [|i1 input]; [ cbn; repeat destruct_pair_let; reflexivity | ].
-  rewrite !fold_left_accumulate_cons_full.
-  cbn [fst snd map step reset_state circuit_state].
-  repeat destruct_pair_let. cbn [fst snd].
-  rewrite <-!surjective_pairing.
-  rewrite fold_left_accumulate_map.
-  rewrite fold_left_accumulate_fold_left_accumulate.
-  cbn [map]. apply f_equal.
-  factor_out_loops.
-  eapply fold_left_accumulate_double_invariant
-    with (I:=fun (x : B * circuit_state c1 * (C * circuit_state c2))
-               (y : C * (circuit_state c1 * circuit_state c2)) =>
-               y = (fst (snd x), (snd (fst x), snd (snd x)))).
-  { reflexivity. }
-  { intros. repeat destruct_pair_let.
-    subst. cbn [fst snd]. reflexivity. }
-  { intros. subst; destruct_products. cbn [fst snd] in *.
-    match goal with H : Forall2 _ _ _ |- _ =>
-                    apply Forall2_eq_map_l in H end.
-    subst. rewrite !map_map. apply map_ext; intros.
-    reflexivity. }
+  simsimpl. generalize (reset_state c2), (reset_state c1).
+  induction input; intros; [ reflexivity | ].
+  simsimpl. rewrite IHinput. reflexivity.
 Qed.
 Hint Rewrite @simulate_compose using solve [eauto] : push_simulate.
 
 Lemma simulate_comb {A B} (c : A -> ident B) (input : list A) :
   simulate (Comb c) input = map c input.
 Proof.
-  clear.
-  cbv [simulate]. destruct input as [|i0 input]; [ reflexivity | ].
-  repeat destruct_pair_let.
-  cbn [fst snd map step reset_state circuit_state].
-  rewrite fold_left_accumulate_to_map.
-  cbn [map fst]. rewrite map_map. cbn [fst].
-  reflexivity.
+  simsimpl. induction input; [ reflexivity | ].
+  simsimpl. rewrite IHinput; reflexivity.
 Qed.
 Hint Rewrite @simulate_comb using solve [eauto] : push_simulate.
 
@@ -86,34 +78,9 @@ Lemma simulate_first {A B C} (f : Circuit A C) (input : list (A * B)) :
   simulate (First f) input = combine (simulate f (map fst input))
                                       (map snd input).
 Proof.
-  clear.
-  cbv [simulate]. destruct input as [|i0 input]; [ reflexivity | ].
-  repeat destruct_pair_let; simpl_ident.
-  cbn [fst snd map step reset_state circuit_state].
-  simpl_ident. repeat destruct_pair_let; simpl_ident.
-  rewrite fold_left_accumulate_map.
-  rewrite !fold_left_accumulate_to_seq with (default:=i0).
-  factor_out_loops.
-  eapply fold_left_accumulate_double_invariant_seq
-    with (I:=fun i x y => y = (fst x, snd (nth i (i0::input) i0), snd x)).
-  { reflexivity. }
-  { intros; subst. destruct_products. cbn [fst snd].
-    repeat destruct_pair_let; simpl_ident.
-    reflexivity. }
-  { intros *. intros ? Hnth; intros.
-    change (snd i0 :: map snd input) with (map snd (i0::input)).
-    subst. cbn [fst snd].
-    eapply list_eq_elementwise; [ length_hammer | ].
-    intros j [c b]; intros.
-    specialize (Hnth j).
-    autorewrite with natsimpl push_length in *.
-    autorewrite with push_nth. destruct_products.
-    let x := constr:(ltac:(eassumption):circuit_state f) in
-    erewrite map_nth_inbounds with (d2:=(c,b,x)) by length_hammer;
-      erewrite map_nth_inbounds with (d2:=(c,x)) by length_hammer.
-    erewrite Hnth by length_hammer. cbn [fst snd].
-    erewrite !map_nth_inbounds by length_hammer.
-    reflexivity. }
+  simsimpl. generalize (reset_state f).
+  induction input; intros; [ reflexivity | ].
+  simsimpl. rewrite IHinput. reflexivity.
 Qed.
 Hint Rewrite @simulate_first using solve [eauto] : push_simulate.
 
@@ -121,86 +88,39 @@ Lemma simulate_second {A B C} (f : Circuit B C) (input : list (A * B)) :
   simulate (Second f) input = combine (map fst input)
                                        (simulate f (map snd input)).
 Proof.
-  clear.
-  cbv [simulate]. destruct input as [|i0 input]; [ reflexivity | ].
-  repeat destruct_pair_let; simpl_ident.
-  cbn [fst snd map step reset_state circuit_state].
-  simpl_ident. repeat destruct_pair_let; simpl_ident.
-  rewrite fold_left_accumulate_map.
-  rewrite !fold_left_accumulate_to_seq with (default:=i0).
-  factor_out_loops.
-  eapply fold_left_accumulate_double_invariant_seq
-    with (I:=fun i x y => y = (fst (nth i (i0::input) i0), fst x, snd x)).
-  { reflexivity. }
-  { intros; subst. destruct_products. cbn [fst snd].
-    repeat destruct_pair_let; simpl_ident.
-    reflexivity. }
-  { intros *. intros ? Hnth; intros.
-    change (fst i0 :: map fst input) with (map fst (i0::input)).
-    subst. cbn [fst snd].
-    eapply list_eq_elementwise; [ length_hammer | ].
-    intros j [a0 c]; intros.
-    specialize (Hnth j).
-    autorewrite with natsimpl push_length in *.
-    autorewrite with push_nth. destruct_products.
-    let x := constr:(ltac:(eassumption):circuit_state f) in
-    erewrite map_nth_inbounds with (d2:=(a0,c,x)) by length_hammer;
-      erewrite map_nth_inbounds with (d2:=(c,x)) by length_hammer.
-    erewrite Hnth by length_hammer. cbn [fst snd].
-    erewrite !map_nth_inbounds by length_hammer.
-    reflexivity. }
+  simsimpl. generalize (reset_state f).
+  induction input; intros; [ reflexivity | ].
+  simsimpl. rewrite IHinput. reflexivity.
 Qed.
 Hint Rewrite @simulate_second using solve [eauto] : push_simulate.
 
 Lemma simulate_DelayInitCE {t} (init : combType t) input :
   simulate (DelayInitCE init) input = firstn (length input)
-                                             (fst (fold_left_accumulate
-                                                     (fun st i_en =>
-                                                        if (snd i_en : bool)
-                                                        then fst i_en
-                                                        else st)
-                                                     input init)).
+                                             (init :: fst (fold_left_accumulate
+                                                            (fun st i_en =>
+                                                               if (snd i_en : bool)
+                                                               then fst i_en
+                                                               else st)
+                                                            input init)).
 Proof.
-  cbv [simulate]. destruct input as [|i0 input]; [ reflexivity | ].
-  repeat destruct_pair_let; simpl_ident.
-  rewrite <-surjective_pairing.
-  autorewrite with push_length push_firstn.
-  rewrite !fold_left_accumulate_to_seq with (default:=i0).
-  cbn [step reset_state]. repeat destruct_pair_let.
-  autorewrite with push_length pull_snoc natsimpl.
-  rewrite fold_left_accumulate_snoc.
-  autorewrite with push_firstn push_length natsimpl listsimpl.
-  factor_out_loops.
-  eapply fold_left_accumulate_double_invariant_seq
-      with (I:=fun i x y => y = (x, if snd (nth i (i0::input) i0)
-                                 then fst (nth i (i0::input) i0)
-                                 else x)).
-  { ssplit; reflexivity. }
-  { cbv zeta; intro i; intros.
-    repeat destruct_pair_let; simpl_ident.
-    destruct_products; cbn [fst snd] in *.
-    logical_simplify; subst. cbn [fst snd].
-    destruct i; autorewrite with push_firstn push_nth listsimpl; reflexivity. }
-  { intros * ?. intro Hnth; intros. subst.
-    cbn [fst snd circuit_state].
-    apply list_eq_elementwise; [ length_hammer | ].
-    intros j d; intros.
-    specialize (Hnth j).
-    autorewrite with natsimpl push_length in *.
-    rewrite !map_nth_inbounds with (d2:=(d,d)) by length_hammer.
-    rewrite Hnth with (da:=d) by length_hammer. cbn [fst snd].
-    reflexivity. }
+  simsimpl. generalize init at 1. generalize init.
+  induction input; intros; [ reflexivity | ].
+  simsimpl. rewrite IHinput.
+  autorewrite with push_length push_firstn push_fold_acc.
+  destruct_products; cbn [fst snd].
+  reflexivity.
 Qed.
 Hint Rewrite @simulate_DelayInitCE using solve [eauto] : push_simulate.
 
 Lemma simulate_DelayCE {t} (input : list (combType t * bool)) :
   simulate DelayCE input = firstn (length input)
-                                  (fst (fold_left_accumulate
-                                          (fun st i_en =>
-                                             if (snd i_en : bool)
-                                             then fst i_en
-                                             else st)
-                                          input defaultSignal)).
+                                  (defaultSignal
+                                     :: fst (fold_left_accumulate
+                                              (fun st i_en =>
+                                                 if (snd i_en : bool)
+                                                 then fst i_en
+                                                 else st)
+                                              input defaultSignal)).
 Proof. apply simulate_DelayInitCE. Qed.
 Hint Rewrite @simulate_DelayCE using solve [eauto] : push_simulate.
 
@@ -211,9 +131,9 @@ Proof.
   erewrite fold_left_accumulate_to_seq with (default:=(defaultSignal,false)).
   eapply fold_left_accumulate_invariant_seq
     with (I:=fun i (st : combType t) acc =>
-               acc = init :: firstn i input
+               acc = firstn i input
                /\ st = nth i (init :: input) defaultSignal).
-  { ssplit; reflexivity. }
+  {  ssplit; reflexivity. }
   { cbv zeta; intro i; intros. subst.
     destruct_products; cbn [fst snd] in *.
     logical_simplify; subst. cbn [fst snd].
@@ -221,7 +141,6 @@ Proof.
     autorewrite with push_firstn push_nth pull_snoc natsimpl.
     rewrite !map_nth_inbounds with (d2:=defaultSignal) by length_hammer.
     erewrite firstn_succ_snoc by lia. cbn [fst snd].
-    rewrite <-app_comm_cons.
     ssplit; reflexivity. }
   { intros. logical_simplify; subst. cbn [fst snd].
     autorewrite with push_length push_firstn.
@@ -237,10 +156,56 @@ Hint Rewrite @simulate_Delay using solve [eauto] : push_simulate.
 Lemma simulate_length {i o} (c : Circuit i o) input :
   length (simulate c input) = length input.
 Proof.
-  cbv [simulate].
-  destruct input; repeat destruct_pair_let; length_hammer.
+  simsimpl. generalize (reset_state c).
+  induction input; intros; [ reflexivity | ].
+  simsimpl. autorewrite with push_length.
+  rewrite IHinput; reflexivity.
 Qed.
 Hint Rewrite @simulate_length using solve [eauto] : push_length.
+
+(* simulate_with_state really SHOULD be fold_left_acc, but we need o for it... any way around this? *)
+Lemma simulate_with_state_snoc i o (c : Circuit i o) st input i0 :
+  simulate_with_state c s (input ++ [i0]) =
+Check simulate_with_state (LoopInitCE _ _).
+Lemma simulate_LoopInitICE_invariant_helper
+      {i s o} resetval (body : Circuit (i * combType s) (o * combType s))
+      (I : nat -> combType s -> circuit_state body ->
+           list o -> list (circuit_state body * combType s) -> Prop)
+      (P : list o * list (circuit_state body * combType s) -> Prop)
+      (start_state : circuit_state body * combType s)
+      (input : list (i * bool)) :
+  (* invariant holds at start *)
+  I 0 (snd start_state) (fst start_state) [] [] ->
+  (* invariant holds through loop *)
+  (forall t out_acc state_acc st bodyst d,
+      I t st bodyst out_acc state_acc ->
+      0 <= t < length input ->
+      let input_en := nth t input d in
+      let out_st'_bodyst' := step body bodyst (fst input_en, st) in
+      let out := fst (fst out_st'_bodyst') in
+      let st' := snd (fst out_st'_bodyst') in
+      let bodyst' := snd out_st'_bodyst' in
+      let new_state := if snd input_en then st' else st in
+      I (S t) new_state bodyst'
+        (out_acc ++ [out])
+        (state_acc ++ [(bodyst', new_state)])) ->
+  (* invariant implies postcondition *)
+  (forall out_acc state_acc st bodyst,
+      I (length input) st bodyst out_acc state_acc ->
+      P (out_acc, state_acc)) ->
+  P (simulate_with_state (LoopInitCE resetval body) start_state input).
+Proof.
+  intros Istart Ipreserved IimpliesP.
+  let sim_result := lazymatch goal with
+                      |- P ?x => x end in
+  rewrite (surjective_pairing sim_result);
+    pose (final_state := last (snd sim_result) start_state).
+  eapply IimpliesP with (st:=snd final_state) (bodyst:=fst final_state).
+  induction input using rev_ind; [ eassumption | ].
+  autorewrite with push_length. rewrite Nat.add_1_r.
+  apply Ipreserved.
+  simsimpl.
+Qed.
 
 Lemma simulate_LoopInitICE_invariant
       {i s o} resetval (body : Circuit (i * combType s) (o * combType s))
@@ -263,6 +228,50 @@ Lemma simulate_LoopInitICE_invariant
   (forall acc st bodyst, I (length input) st bodyst acc -> P acc) ->
   P (simulate (LoopInitCE resetval body) input).
 Proof.
+  intros Istart Ipreserved IimpliesP.
+  simsimpl.
+  (* get the list of states *)
+  lazymatch goal with
+  | |- context [simulate-
+  pose (snd 
+  pose (fold_left (fun st i_en =>
+                     let x := step body (fst st) (fst i_en, snd st) in
+                     (snd x, if (snd i_en : bool) then snd (fst x) else snd st))
+                  input (reset_state body, resetval)) as final_state.
+  apply IimpliesP with (st:=snd final_state) (bodyst:=fst final_state).
+  subst final_state.
+  generalize resetval at 3.
+  generalize dependent (reset_state body).
+  generalize dependent resetval.
+  induction input; intros; [ eassumption | ].
+  simsimpl. autorewrite with push_length.
+  destruct_products. cbn [fst snd fold_left].
+  eapply Ipreserved.
+  rewrite IHinput.
+  generalize resetval at 1.
+  generalize (reset_state body), resetval.
+  induction input; intros; [ solve [eauto] | ].
+  simsimpl.
+  1:cbn.
+  1:eauto.
+  destruct input; [ solve [eauto] | ].
+  repeat destruct_pair_let.
+  cbn [circuit_state reset_state step fst snd].
+  apply fold_left_accumulate_invariant_seq
+    with (I0:=fun t '(out,(bodyst,st)) acc =>
+                I (S t) st bodyst (map fst acc));
+    intros *; repeat destruct_pair_let; cbn [fst snd].
+  { specialize (Ipreserved 0 []). cbn [nth app length] in Ipreserved.
+    cbn [map fst snd]. eapply Ipreserved; eauto; [ ]. Lia.lia. }
+  { intros. specialize (Ipreserved (S t)).
+    autorewrite with pull_snoc.
+    eapply Ipreserved; eauto; [ ].
+    cbn [combType] in *; length_hammer. }
+  { eapply IimpliesP. }
+
+
+
+  
   intros ? Ipreserved IimpliesP. cbv [simulate].
   destruct input; [ solve [eauto] | ].
   repeat destruct_pair_let.
